src/examples/TripleExamples.v
@@ -1,0 +1,9 @@
+From mathcomp Require Import all_ssreflect.
+Set Implicit Arguments.
+Unset Strict Implicit.
+Unset Printing Implicit Defensive.
+From RDF Require Import Triple Term.
+
+
+(* Definition s :=  *)
+(* show example term \in triple *)
